\documentclass[12pt, final]{article}
\usepackage{color}
\usepackage{times}
\usepackage{amssymb,amsmath,amsthm}
\usepackage{dsfont}
\usepackage{graphicx}
\usepackage{enumerate}
\usepackage{enumitem}
\usepackage[paperwidth=8.5in,left=1.0in,right=1.0in,top=1.0in,bottom=1.0in,paperheight=11.0in]{geometry}
\usepackage[labelsep=colon,singlelinecheck=false,footnotesize]{caption}
\usepackage{fancyhdr}
\usepackage{float}
\usepackage{booktabs}
\usepackage[sort&compress]{natbib}
\usepackage{subfig}
\usepackage{titlesec}
\usepackage[breaklinks]{hyperref}
\hypersetup{pdfdisplaydoctitle=true,bookmarksnumbered=true,colorlinks=true,citecolor=black,linkcolor=darkblue,urlcolor=darkred,pdfstartview=FitH,pdfpagemode=UseNone}
\usepackage[hyphenbreaks]{breakurl}
\usepackage{accents}
\newcommand{\ubar}[1]{\underaccent{\bar}{#1}}


%Define Color Names
\definecolor{Gray}{rgb}{0.65,0.65,0.65}
\definecolor{darkblue}{rgb}{0,0,0.55}
\definecolor{darkred}{rgb}{0.5,0,0}

%Section Headings
\newcommand\Bheadfont{\fontsize{14pt}{\baselineskip}\selectfont}
\titleformat{\section}[hang]{\normalfont\sc\color{darkblue}\Bheadfont}{\thesection\hskip0.618em}{0em}{}
\titlespacing*{\section}{0pt}{15pt plus 2pt minus 2pt}{9pt plus 2pt minus 2pt}
\titleformat{\subsection}[runin]{\normalfont\sc\color{darkblue}} {\thesubsection\hskip0.618em}{0em}{}
\titlespacing*{\subsection}{0pt}{13pt plus 2pt minus 2pt}{13pt plus 2pt minus 2pt}
\titleformat{\subsubsection}[runin]{\normalfont\sc\color{darkblue}} {\thesubsubsection\hskip0.618em}{0em}{}
\titlespacing*{\subsubsection}{0pt}{13pt plus 2pt minus 2pt}{13pt plus 2pt minus 2pt}
\titleformat{\paragraph}[runin]{\bfseries}{\theparagraph\hskip0.618em}{0em}{}
\titlespacing*{\paragraph}{0pt}{13pt plus 2pt minus 2pt}{13pt plus 2pt minus 2pt}

\begin{document}

\section{Equilibrium System}

\noindent Preferences:
\begin{gather*}
  E_0\textstyle\sum_{t=0}^\infty\beta^t a_t[\log(c_t)-\chi n_t^{1+\eta}/(1+\eta)]
\end{gather*}

\noindent Budget Constraint:
\begin{gather*}
  c_t+b_t/(i_t\bar{s})=w_tn_t+b_{t-1}/\pi_t+d_t
\end{gather*}

\setcounter{equation}{0}
\subsection{ART Model}
\noindent Equilibrium system (11 equations):
\small\begin{gather}
c_t = [1-\varphi(\pi_t^{gap}-1)^2/2]y_t\\
i_t^*=(i^*_{t-1})^{\rho_i}(\bar{\imath}(\pi^{gap}_t)^{\phi_\pi})^{1-\rho_i}\exp(\sigma_\nu\nu_t)\\
i_t=\max\{1,i_t^*\}\\
\lambda_t = c_t \\
w_t = \chi n_t^\eta \lambda_t\\
1 =  \beta E_t[(\lambda_t/\lambda_{t+1})(s_ti_t/(\bar{\pi}\pi_{t+1}^{gap}g_{t+1}))]\\
\varphi(\pi_t^{gap}-1)\pi_t^{gap} = 1-\theta + \theta w_t/z_t + \beta\varphi E_t[(\lambda_t/\lambda_{t+1})(\pi_{t+1}^{gap}-1)\pi_{t+1}^{gap}(y_{t+1}/y_t)]\\
  y_t=z_t n_t\\  
  g_t= (1-\rho_g)\bar{g}+\rho_gg_{t-1} + \sigma_\varepsilon\varepsilon_t \\
  s_t=(1-\rho_s)\bar{s}+\rho_ss_{t-1} + \sigma_\upsilon\upsilon_t\\
  z_t=g_tz_{t-1}
\end{gather}\normalsize
Variables: $\{c,i^*,i,\lambda,w,\pi^{gap},y,n,g,s,z\}$\\

\setcounter{equation}{0}
\noindent De-trended Equilibrium System (10 equations):
\small\begin{gather}
\tilde{c}_t = [1-\varphi(\pi_t^{gap} - 1)^2/2]\tilde{y}_t\\
i_t^*=(i^*_{t-1})^{\rho_i}(\bar{\imath}(\pi_t^{gap})^{\phi_\pi})^{1-\rho_i}\exp(\sigma_\nu\nu_t)\\
i_t=\max\{1,i_t^*\}\\
\tilde{\lambda}_t = \tilde{c}_t\\
\tilde{w}_t = \chi n_t^\eta \tilde{\lambda}_t  \\
  1 = \beta E_t[(\tilde{\lambda}_t/\tilde{\lambda}_{t+1})(s_ti_t/(\bar{\pi}\pi_{t+1}^{gap}g_{t+1}))]\\
  \varphi(\pi_t^{gap}-1){\pi}_t^{gap} = 1-\theta + \theta\tilde{w}_t + \beta\varphi E_t[(\tilde{\lambda}_t/\tilde{\lambda}_{t+1}) (\pi_{t+1}^{gap}-1)\pi_{t+1}^{gap}(\tilde{y}_{t+1}/\tilde{y}_t)]\\
  \tilde{y}_t= n_t\\  
  g_t= (1-\rho_g)\bar{g}+\rho_gg_{t-1} + \sigma_\varepsilon\varepsilon_t \\
  s_t=(1-\rho_s)s_t+\rho_ss_{t-1} + \sigma_\upsilon\upsilon_t
\end{gather}
Variables: $\{\tilde{c},i^*,i,\tilde{\lambda},\tilde{w},\pi^{gap},\tilde{y},n,g,s,z\}$\\ 

\setcounter{equation}{0}
\noindent Log-linear Equilibrium System:
\begin{gather}
  \hat{c}_t = \hat{y}_t\\
  \hat{\imath}_t^n = \rho_i\hat{\imath}^n_{t-1} + (1-\rho_i)\phi_\pi\hat{\pi}_t+\sigma_\nu\nu_t \\
  \hat{\imath}_t = \hat{\imath}_t^n\\
  \hat{\lambda}_t = \hat{c}_t \\
  \hat{w}_t =  \eta\hat{n}_t + \hat{\lambda}_t\\
  \hat{\lambda}_t + \hat{\imath}_t + s_t  = E_t\hat{\lambda}_{t+1}+E_t\hat{\pi}_{t+1} \\
  \varphi\hat{\pi}_t = (\theta-1)\hat{w}_t+\beta\varphi E_t\hat{\pi}_{t+1}\\
  \hat{y}_t = \hat{n}_t 
\end{gather}
\pagebreak
\setcounter{equation}{0}
\subsection{Gust Et Al Model}
\noindent Equilibrium system (13 equations):
\small\begin{gather}
c_t = [1-\varphi(\pi_t^{gap}-1)^2/2]y_t\\
i_t^*=(i^*_{t-1})^{\rho_i}(\bar{\imath}(\pi^{gap}_t)^{\phi_\pi})^{1-\rho_i}\exp(\sigma_\nu\nu_t)\\
i_t=\max\{1,i_t^*\}\\
\lambda_t = c_t \\
w_t = \chi n_t^\eta \lambda_t\\
V_{\lambda,t} =  \beta E_t[(1/\lambda_{t+1})(s_ti_t/(\bar{\pi}\pi_{t+1}^{gap}g_{t+1}))]\\
1/\lambda_t = V_{\lambda,t}\\
V_{\pi,t} = 1-\theta + \theta w_t/z_t + \beta\varphi E_t[(\lambda_t/\lambda_{t+1})(\pi_{t+1}^{gap}-1)\pi_{t+1}^{gap}(y_{t+1}/y_t)]\\
\varphi(\pi_t^{gap}-1)\pi_t^{gap} = V_{\pi,t}\\
%1 =  \beta E_t[(\lambda_t/\lambda_{t+1})(s_ti_t/(\bar{\pi}\pi_{t+1}^{gap}g_{t+1}))]\\
%\varphi(\pi_t^{gap}-1)\pi_t^{gap} = 1-\theta + \theta w_t/z_t + \beta\varphi E_t[(\lambda_t/\lambda_{t+1})(\pi_{t+1}^{gap}-1)\pi_{t+1}^{gap}(y_{t+1}/y_t)]\\
  y_t=z_t n_t\\  
  g_t= (1-\rho_g)\bar{g}+\rho_gg_{t-1} + \sigma_\varepsilon\varepsilon_t \\
  s_t=(1-\rho_s)\bar{s}+\rho_ss_{t-1} + \sigma_\upsilon\upsilon_t\\
  z_t=g_tz_{t-1}
\end{gather}\normalsize
Variables: $\{c,i^*,i,\lambda,w,\pi^{gap},V_{\lambda},y,V_{\pi},n,g,s,z\}$\\

\setcounter{equation}{0}
\noindent De-trended Equilibrium System (12 equations):
\small\begin{gather}
\tilde{c}_t = [1-\varphi(\pi_t^{gap} - 1)^2/2]\tilde{y}_t\\
i_t^*=(i^*_{t-1})^{\rho_i}(\bar{\imath}(\pi_t^{gap})^{\phi_\pi})^{1-\rho_i}\exp(\sigma_\nu\nu_t)\\
i_t=\max\{1,i_t^*\}\\
\tilde{\lambda}_t = \tilde{c}_t\\
\tilde{w}_t = \chi n_t^\eta \tilde{\lambda}_t  \\
  %1 = \beta E_t[(\tilde{\lambda}_t/\tilde{\lambda}_{t+1})(s_ti_t/(\bar{\pi}\pi_{t+1}^{gap}g_{t+1}))]\\ %rewrite in terms of V_\lambda
%\varphi(\pi_t^{gap}-1)\hat{\pi}_t^{gap} = 1-\theta + \theta\tilde{w}_t + \beta\varphi E_t[(\tilde{\lambda}_t/\tilde{\lambda}_{t+1}) (\pi_{t+1}^{gap}-1)\pi_{t+1}^{gap}(\tilde{y}_{t+1}/\tilde{y}_t)]\\ %rewrite in terms of V_\pi
\tilde{V}_{\lambda,t} = \beta E_t[(1/\tilde{\lambda}_{t+1})(s_ti_t/(\bar{\pi}\pi^{gap}_{t+1}g_{t+1}))]\\%
1/\tilde{\lambda}_t = \tilde{V}_{\lambda,t}\\%
\tilde{V}_{\pi_t} = 1 - \theta + \theta\tilde{w}_t + \beta\varphi E_t[(\tilde{\lambda}_t/\tilde{\lambda}_{t+1})(\pi^{gap}_{t+1}-1)\pi^{gap}_{t+1}(\tilde{y}_{t+1}/\tilde{y}_t)]\\
\varphi(\pi_t^{gap}-1){\pi}_t^{gap} = \tilde{V}_{\pi,t}\\
  \tilde{y}_t= n_t\\  
  g_t= (1-\rho_g)\bar{g}+\rho_gg_{t-1} + \sigma_\varepsilon\varepsilon_t \\
  s_t=(1-\rho_s)s_t+\rho_ss_{t-1} + \sigma_\upsilon\upsilon_t
\end{gather}
Variables: $\{\tilde{c},i^*,i,\tilde{\lambda},\tilde{w},\pi^{gap},\tilde{V}_{\lambda},\tilde{y},\tilde{V}_{\pi},n,g,s,z\}$\\ 

\setcounter{equation}{0}
\noindent Log-linear Equilibrium System:
\begin{gather}
  \hat{c}_t = \hat{y}_t\\
  \hat{\imath}_t^n = \rho_i\hat{\imath}^n_{t-1} + (1-\rho_i)\phi_\pi\hat{\pi}_t+\sigma_\nu\nu_t \\
  \hat{\imath}_t = \hat{\imath}_t^n\\
  \hat{\lambda}_t = \hat{c}_t \\
  \hat{w}_t =  \eta\hat{n}_t + \hat{\lambda}_t\\
  \hat{V}_{\lambda,t} =  \hat{\imath}_t + s_t - E_t\hat{\lambda}_{t+1} - E_t\hat{\pi}_{t+1} \\
  -\hat{\lambda}_t = \hat{V}_{\lambda,t} \\
  %\hat{\lambda}_t + \hat{\imath}_t + s_t  = E_t\hat{\lambda}_{t+1}+E_t\hat{\pi}_{t+1} \\
  \hat{V}_{\pi,t} = (\theta-1)\hat{w}_t+\beta\varphi E_t\hat{\pi}_{t+1}\\
  \varphi\hat{\pi}_t = \hat{V}_{\pi,t}\\
  %\varphi\hat{\pi}_t = (\theta-1)\hat{w}_t+\beta\varphi E_t\hat{\pi}_{t+1}\\ 
  \hat{y}_t = \hat{n}_t 
\end{gather}

\end{document}

