\documentclass[12pt, final]{article}
\usepackage{color}
\usepackage{times}
\usepackage{amssymb,amsmath,amsthm}
\usepackage{comment}
\usepackage{dsfont}
\usepackage{graphicx}
\usepackage{enumerate}
\usepackage{enumitem}
\usepackage[paperwidth=8.5in,left=1.0in,right=1.0in,top=1.0in,bottom=1.0in,paperheight=11.0in]{geometry}
\usepackage[labelsep=colon,singlelinecheck=false,footnotesize]{caption}
\usepackage{fancyhdr}
\usepackage{float}
\usepackage{booktabs}
\usepackage[sort&compress]{natbib}
\usepackage{subfig}
\usepackage{titlesec}
\usepackage[breaklinks]{hyperref}
\hypersetup{pdfdisplaydoctitle=true,bookmarksnumbered=true,colorlinks=true,citecolor=black,linkcolor=darkblue,urlcolor=darkred,pdfstartview=FitH,pdfpagemode=UseNone}
\usepackage[hyphenbreaks]{breakurl}
\usepackage{accents}
\newcommand{\ubar}[1]{\underaccent{\bar}{#1}}


%Define Color Names
\definecolor{Gray}{rgb}{0.65,0.65,0.65}
\definecolor{darkblue}{rgb}{0,0,0.55}
\definecolor{darkred}{rgb}{0.5,0,0}

%Section Headings
\newcommand\Bheadfont{\fontsize{14pt}{\baselineskip}\selectfont}
\titleformat{\section}[hang]{\normalfont\sc\color{darkblue}\Bheadfont}{\thesection\hskip0.618em}{0em}{}
\titlespacing*{\section}{0pt}{15pt plus 2pt minus 2pt}{9pt plus 2pt minus 2pt}
\titleformat{\subsection}[runin]{\normalfont\sc\color{darkblue}} {\thesubsection\hskip0.618em}{0em}{}
\titlespacing*{\subsection}{0pt}{13pt plus 2pt minus 2pt}{13pt plus 2pt minus 2pt}
\titleformat{\subsubsection}[runin]{\normalfont\sc\color{darkblue}} {\thesubsubsection\hskip0.618em}{0em}{}
\titlespacing*{\subsubsection}{0pt}{13pt plus 2pt minus 2pt}{13pt plus 2pt minus 2pt}
\titleformat{\paragraph}[runin]{\bfseries}{\theparagraph\hskip0.618em}{0em}{}
\titlespacing*{\paragraph}{0pt}{13pt plus 2pt minus 2pt}{13pt plus 2pt minus 2pt}

\begin{document}

\section{Equilibrium System}

\subsection{ART Model with capital}
\noindent Preferences:
\begin{gather*}
  E_0\textstyle\sum_{t=0}^\infty\beta^t [\log(c_t-hc^a_{t-1})-\chi n_t^{1+\eta}/(1+\eta)]
\end{gather*}

\noindent Budget Constraint:
\begin{gather*}
  c_t+x_t+b_t/(i_ts_t)=w_tn_t+r_t^kk_{t-1}+b_{t-1}/\pi_t+d_t\\
  k_t = (1-\delta)k_{t-1} + x_t(1 - \nu(x^g_t-1)^2/2)
\end{gather*}

\setcounter{equation}{0}
\noindent Equilibrium system:
\small\begin{gather}
y_t = k_{t-1}^\alpha(z_t n_t)^{1-\alpha}\\ %%%
r_t^k = \alpha mc_ty_t/k_{t-1}\\
w_t = (1-\alpha)mc_ty_t/n_t\\
%w_t^g = \pi_tw_t(\bar{\pi}gw_{t-1})\\
y_t^{gdp} = [1 - \varphi(\pi_t^{gap}-1)^2/2]y_t \\
y^g_t = y^{gdp}_t/(\bar{g}y^{gdp}_{t-1})\\
i_t^*=(i^*_{t-1})^{\rho_i}(\bar{\imath}(\pi^{gap}_t)^{\phi_\pi}(y^{g}_{t})^{\phi_y})^{1-\rho_i}\exp(mp_t)\\
i_t=\max\{1,i_t^*\}\\
\lambda_t = c_t - hc^a_{t-1} \\
w_t = \chi n_t^\eta \lambda_t\\
c_t + x_t = y_t^{gdp}\\
x_t^g = x_t/(\bar{g}x_{t-1})\\
k_t = (1-\delta)k_{t-1}+x_t(1-\nu(x_t^g-1)^2/2) \\%%%
1 =  \beta E_t[(\lambda_t/\lambda_{t+1})(s_ti_t/(\bar{\pi}\pi_{t+1}^{gap}))]\\
q_t = \beta E_t[(\lambda_t/\lambda_{t+1})(r^k_{t+1}+(1-\delta)q_{t+1})]\\
1 = q_t[1-\nu(x^g_t-1)^2/2 - \nu(x_t^g-1)x_t^g] + \nu\beta\bar{g}E_t[q_{t+1}(\lambda_t/\lambda_{t+1})(x^g_{t+1})^2(x^g_{t+1}-1)]\\
\varphi(\pi_t^{gap}-1)\pi_t^{gap} = 1-\theta + \theta mc_t + \beta\varphi E_t[(\lambda_t/\lambda_{t+1})(\pi_{t+1}^{gap}-1)\pi_{t+1}^{gap}(y_{t+1}/y_t)]\\
g_t = \bar{g} + \sigma_g\varepsilon_{g,t}\\
s_t=(1-\rho_s)\bar{s}+\rho_ss_{t-1} + \sigma_s\varepsilon_{s,t}\\
mp_t = \sigma_i\varepsilon_{i,t}\\
  z_t=g_tz_{t-1}
\end{gather}\normalsize
Variables: $\{c,n,x,k,y^{gdp},y,x^g,y^g,w,r^k,\pi,i,i^n,q,mc,\lambda,g,s,mp,z\}$\\

\setcounter{equation}{0}
\noindent De-trended Equilibrium System:
\small\begin{gather}
\tilde{y}_t= (\tilde{k}_{t-1}/g_t)^\alpha n_t^{1-\alpha}\\
r^k_t = \alpha mc_t g_t \tilde{y}_t/\tilde{k}_{t-1}\\
\tilde{w}_t = (1-\alpha)mc_t\tilde{y}_t/n_t\\
\tilde{y}^{gdp}_t = [1-\varphi(\pi_t^{gap} - 1)^2/2]\tilde{y}_t\\
y^g_t = g_t\tilde{y}^{gdp}_t/(\bar{g}\tilde{y}^{gdp}_{t-1})\\
i_t^*=(i^*_{t-1})^{\rho_i}(\bar{\imath}(\pi_t^{gap})^{\phi_\pi}(y^g_t)^{\phi_y})^{1-\rho_i}\exp(\sigma_i\varepsilon_{i,t})\\
i_t=\max\{1,i_t^*\}\\
\tilde{\lambda}_t = \tilde{c}_t\ - h\tilde{c}_{t-1}/g_t\\
\tilde{w}_t = \chi n_t^\eta \tilde{\lambda}_t  \\
\tilde{c}_t + \tilde{x}_t = \tilde{y}^{gdp}_t\\
x^g_t = g_t\tilde{x}_t/(\bar{g}\tilde{x}_{t-1})\\
\tilde{k}_t = (1-\delta)(\tilde{k}_{t-1}/g_t) + \tilde{x}_t(1-\nu(x^g_t-1)^2/2)\\%%%
  1 = \beta E_t[(\tilde{\lambda}_t/\tilde{\lambda}_{t+1})(s_ti_t/(\bar{\pi}\pi_{t+1}^{gap}g_{t+1}))]\\
q_t = \beta E_t[(\tilde{\lambda}_t/\tilde{\lambda}_{t+1})(r^k_{t+1} + (1-\delta)q_{t+1})/g_{t+1}]\\
1 = q_t[1 - \nu(x^g_t-1)^2/2 - \nu(x^g_t-1)x^g_t] + \nu\beta\bar{g}E_t[q_{t+1}(\tilde{\lambda}_t/\tilde{\lambda}_{t+1})(x^g_{t+1})^2(x^g_{t+1}-1)/g_{t+1}]\\
  \varphi(\pi_t^{gap}-1){\pi}_t^{gap} = 1-\theta + \theta mc_t + \beta\varphi E_t[(\tilde{\lambda}_t/\tilde{\lambda}_{t+1}) (\pi_{t+1}^{gap}-1)\pi_{t+1}^{gap}(\tilde{y}_{t+1}/\tilde{y}_t)]\\
  g_t= \bar{g} + \sigma_g\varepsilon_{g,t} \\
  s_t=(1-\rho_s)s_t+\rho_ss_{t-1} + \sigma_s\varepsilon_{s,t}\\
  mp_t = \sigma_i\varepsilon_{i,t}
\end{gather}
Variables:$\{\tilde{c},\tilde{n},\tilde{x},\tilde{k},\tilde{y^{gdp}},\tilde{y},x^g,y^g,\tilde{w},r^k,\pi,i,i^n,q,mc,\tilde{\lambda},g,s,mp\}$\\

\setcounter{equation}{0}
\noindent Log-linear Equilibrium System:
\begin{gather}
  \hat{y}_t/\bar{y} = \alpha(\hat{k}_{t-1}/\bar{k} - \hat{g}_t/\bar{g}) + (1-\alpha)\hat{n}_t/\bar{n}\\
\hat{r}^k_t/\bar{r}^k = \hat{mc}_t/\bar{mc} + \hat{g}_t/\bar{g} + \hat{y}_t/\bar{y} - \hat{k}_{t-1}/\bar{k}\\
\hat{w}_t/\bar{w} = \hat{mc}_t/\bar{mc} + \hat{y}_t/\bar{y} - \hat{n}_t/\bar{n}\\
\hat{y}_t^{gdp} = \hat{y}_t\\
\hat{y}^g_t = \hat{g}_t/\bar{g} + \hat{y}^{gdp}_t/\bar{y}^{gdp} - \hat{y}^{gdp}_{t-1}/\bar{y}^{gdp}\\
  \hat{i}_t/\bar{i} = \rho_i\hat{i}_{t-1}/\bar{i} + (1-\rho_i)(\phi_\pi\hat{\pi}^{gap}_t+ \phi_y\hat{y}^g_t)+\hat{mp}_t \\
  \hat{\imath}_t = \hat{\imath}_t^n\\
  \hat{\lambda}_t = \hat{c}_t - (h/\bar{g})\hat{c}_{t-1} + (h\bar{c}/\bar{g}^2)\hat{g}_t\\
  \hat{c}_t + \hat{x}_t = \hat{y}^{gdp}_t\\
  \hat{x}^g_t = \hat{g}_t/\bar{g} + \hat{x}_t/\bar{x} - \hat{x}_{t-1}/\bar{x}\\
  \hat{k}_t = ((1-\delta)/\bar{g})[\hat{k}_{t-1}-(\bar{k}/\bar{g})\hat{g}_t] + \hat{x}_t\\
  \hat{\lambda}_t/\bar{\lambda} + \hat{\imath}_t/\bar{i} + \hat{s}_t/\bar{s}  = E_t\hat{\lambda}_{t+1}/\bar{\lambda}+E_t\hat{g}_{t+1}/\bar{g}+E_t\hat{\pi}_{t+1}/\bar{\pi} \\
  \hat{q}_t = \hat{\lambda}_t/\bar{\lambda} - E_t\hat{\lambda}_{t+1}/\bar{\lambda} + (\beta/\bar{g})[E_t\hat{r}^k_{t+1} + (1-\delta)E_t\hat{q}_{t+1}] - E_t\hat{g}_{t+1}/\bar{g}\\
  \hat{x}^g_t = \hat{q}_t + \beta E_t\hat{x}^g_{t+1}\\
  \varphi\hat{\pi}^{gap}_t = \theta\hat{mc}_t+\beta\varphi E_t\hat{\pi}^{gap}_{t+1}\\
  \hat{g}_t = \sigma_g\varepsilon_{g,t}\\
  \hat{s}_t = \rho_s\hat{s}_{t-1} + \sigma_s\varepsilon_{s,t}\\
  \hat{mp}_t = \sigma_i\varepsilon_{i,t}
\end{gather}
Variables:$\{\hat{c},\hat{n},\hat{x},\hat{k},\hat{y^{gdp}},\hat{y},\hat{x^g},\hat{y^g},\hat{w},\hat{r^k},\hat{\pi},\hat{i},\hat{i^n},\hat{q},\hat{\lambda},\hat{g},\hat{s},\hat{mp}\}$\\
\begin{comment}
\pagebreak









\subsection{ART Model pre-capital}
\noindent Preferences:
\begin{gather*}
  E_0\textstyle\sum_{t=0}^\infty\beta^t [\log(c_t-hc^a_{t-1})-\chi n_t^{1+\eta}/(1+\eta)]
\end{gather*}

\noindent Budget Constraint:
\begin{gather*}
  c_t+b_t/(i_ts_t)=w_tn_t+b_{t-1}/\pi_t+d_t
\end{gather*}

\setcounter{equation}{0}
\noindent Equilibrium system (11 equations):
\small\begin{gather}
c_t = [1-\varphi(\pi_t^{gap}-1)^2/2]y_t\\
i_t^*=(i^*_{t-1})^{\rho_i}(\bar{\imath}(\pi^{gap}_t)^{\phi_\pi}(c_t/(\bar{g}c_{t-1}))^{\phi_c})^{1-\rho_i}\exp(\sigma_\nu\nu_t)\\
i_t=\max\{1,i_t^*\}\\
\lambda_t = c_t - hc^a_{t-1} \\
w_t = \chi n_t^\eta \lambda_t\\
1 =  \beta E_t[(\lambda_t/\lambda_{t+1})(s_ti_t/(\bar{\pi}\pi_{t+1}^{gap}))]\\
\varphi(\pi_t^{gap}-1)\pi_t^{gap} = 1-\theta + \theta w_t/z_t + \beta\varphi E_t[(\lambda_t/\lambda_{t+1})(\pi_{t+1}^{gap}-1)\pi_{t+1}^{gap}(y_{t+1}/y_t)]\\
  y_t=z_t n_t\\  
  g_t= (1-\rho_g)\bar{g}+\rho_gg_{t-1} + \sigma_\varepsilon\varepsilon_t \\
  s_t=(1-\rho_s)\bar{s}+\rho_ss_{t-1} + \sigma_\upsilon\upsilon_t\\
  z_t=g_tz_{t-1}
\end{gather}\normalsize
Variables: $\{c,i^*,i,\lambda,w,\pi^{gap},y,n,g,s,z\}$\\

\setcounter{equation}{0}
\noindent De-trended Equilibrium System (10 equations):
\small\begin{gather}
\tilde{c}_t = [1-\varphi(\pi_t^{gap} - 1)^2/2]\tilde{y}_t\\
i_t^*=(i^*_{t-1})^{\rho_i}(\bar{\imath}(\pi_t^{gap})^{\phi_\pi}(g_t\tilde{c}_t/(\bar{g}\tilde{c}_{t-1})^{\phi_c})^{1-\rho_i}\exp(\sigma_\nu\nu_t)\\
i_t=\max\{1,i_t^*\}\\
\tilde{\lambda}_t = \tilde{c}_t\ - h\tilde{c}_{t-1}/g_t\\
\tilde{w}_t = \chi n_t^\eta \tilde{\lambda}_t  \\
  1 = \beta E_t[(\tilde{\lambda}_t/\tilde{\lambda}_{t+1})(s_ti_t/(\bar{\pi}\pi_{t+1}^{gap}g_{t+1}))]\\
  \varphi(\pi_t^{gap}-1){\pi}_t^{gap} = 1-\theta + \theta\tilde{w}_t + \beta\varphi E_t[(\tilde{\lambda}_t/\tilde{\lambda}_{t+1}) (\pi_{t+1}^{gap}-1)\pi_{t+1}^{gap}(\tilde{y}_{t+1}/\tilde{y}_t)]\\
  \tilde{y}_t= n_t\\  
  g_t= (1-\rho_g)\bar{g}+\rho_gg_{t-1} + \sigma_\varepsilon\varepsilon_t \\
  s_t=(1-\rho_s)s_t+\rho_ss_{t-1} + \sigma_\upsilon\upsilon_t
\end{gather}
Variables: $\{\tilde{c},i^*,i,\tilde{\lambda},\tilde{w},\pi^{gap},\tilde{y},n,k,g,s\}$\\ 

\setcounter{equation}{0}
\noindent Log-linear Equilibrium System:
\begin{gather}
  \hat{c}_t = \hat{y}_t\\
  \hat{\imath}_t^n = \rho_i\hat{\imath}^n_{t-1} + (1-\rho_i)\phi_\pi\hat{\pi}_t+ (1-\rho_i)\phi_c(\hat{g}+\hat{c}-\hat{c}_{t-1})+\sigma_\nu\nu_t \\
  \hat{\imath}_t = \hat{\imath}_t^n\\
  (1-h/g)\hat{\lambda}_t = \hat{c}_t + (h/g)(\hat{g} - \hat{c}_{t-1})\\
  \hat{w}_t =  \eta\hat{n}_t + \hat{\lambda}_t\\
  \hat{\lambda}_t + \hat{\imath}_t + s_t  = E_t\hat{\lambda}_{t+1}+E_t\hat{\pi}_{t+1} \\
  \varphi\hat{\pi}_t = (\theta-1)\hat{w}_t+\beta\varphi E_t\hat{\pi}_{t+1}\\
  \hat{y}_t = \hat{n}_t 
\end{gather}
\pagebreak
\setcounter{equation}{0}
\subsection{Gust Et Al Model}
\noindent Equilibrium system (13 equations):
\small\begin{gather}
\varphi(\pi_t^{gap}-1)\pi_t^{gap} = 1-\theta + \theta w_t/z_t + \beta\varphi E_t[(\lambda_t/\lambda_{t+1})(\pi_{t+1}^{gap}-1)\pi_{t+1}^{gap}(y_{t+1}/y_t)]\\
i_t^*=(i^*_{t-1})^{\rho_i}(\bar{\imath}(\pi^{gap}_t)^{\phi_\pi})^{1-\rho_i}\exp(\sigma_\nu\nu_t)\\
i_t=\max\{1,i_t^*\}\\
1/\lambda_t =  \beta E_t[(1/\lambda_{t+1})(s_ti_t/(\bar{\pi}\pi_{t+1}^{gap}g_{t+1}))]\\
\lambda_t = c_t \\
c_t = [1-\varphi(\pi_t^{gap}-1)^2/2]y_t\\
w_t = \chi n_t^\eta \lambda_t\\
  y_t=z_t n_t\\  
  g_t= (1-\rho_g)\bar{g}+\rho_gg_{t-1} + \sigma_\varepsilon\varepsilon_t \\
  s_t=(1-\rho_s)\bar{s}+\rho_ss_{t-1} + \sigma_\upsilon\upsilon_t\\
  z_t=g_tz_{t-1}
\end{gather}\normalsize
Variables: $\{c,i^*,i,\lambda,w,\pi^{gap},V_{\lambda},y,V_{\pi},n,g,s,z\}$\\

\setcounter{equation}{0}
\noindent De-trended Equilibrium System (12 equations):
\small\begin{gather}
\varphi(\pi_t^{gap}-1){\pi}_t^{gap} = 1 - \theta + \theta\tilde{w}_t + \beta\varphi E_t[(\tilde{\lambda}_t/\tilde{\lambda}_{t+1})(\pi^{gap}_{t+1}-1)\pi^{gap}_{t+1}(\tilde{y}_{t+1}/\tilde{y}_t)]\\
i_t^*=(i^*_{t-1})^{\rho_i}(\bar{\imath}(\pi_t^{gap})^{\phi_\pi})^{1-\rho_i}\exp(\sigma_\nu\nu_t)\\
i_t=\max\{1,i_t^*\}\\
1/\tilde{\lambda}_t = \beta E_t[(1/\tilde{\lambda}_{t+1})(s_ti_t/(\bar{\pi}\pi^{gap}_{t+1}g_{t+1}))]\\%
\tilde{\lambda}_t = \tilde{c}_t\\
\tilde{c}_t = [1-\varphi(\pi_t^{gap} - 1)^2/2]\tilde{y}_t\\
\tilde{w}_t = \chi n_t^\eta \tilde{\lambda}_t  \\
  \tilde{y}_t= n_t\\  
  g_t= (1-\rho_g)\bar{g}+\rho_gg_{t-1} + \sigma_\varepsilon\varepsilon_t \\
  s_t=(1-\rho_s)s_t+\rho_ss_{t-1} + \sigma_\upsilon\upsilon_t
\end{gather}
Variables: $\{\tilde{c},i^*,i,\tilde{\lambda},\tilde{w},\pi^{gap},\tilde{V}_{\lambda},\tilde{y},\tilde{V}_{\pi},n,g,s\}$\\ 

\setcounter{equation}{0}
\noindent Log-linear Equilibrium System:
\begin{gather}
  \varphi\hat{\pi}_t = (\theta-1)\hat{w}_t+\beta\varphi E_t\hat{\pi}_{t+1}\\
  \hat{\imath}_t^n = \rho_i\hat{\imath}^n_{t-1} + (1-\rho_i)\phi_\pi\hat{\pi}_t+\sigma_\nu\nu_t \\
  \hat{\imath}_t = \hat{\imath}_t^n\\
    -\hat{\lambda}_t = \hat{\imath}_t + s_t - E_t\hat{\lambda}_{t+1} - E_t\hat{\pi}_{t+1} \\
  \hat{\lambda}_t = \hat{c}_t \\
  \hat{c}_t = \hat{y}_t\\
  \hat{w}_t =  \eta\hat{n}_t + \hat{\lambda}_t\\
  \hat{y}_t = \hat{n}_t
\end{gather}

\setcounter{equation}{0}
\noindent Gust et al Indicator Functions\\
\begin{gather}
  c_{t+1,1} = \beta E_t[\lambda_t(s_ti_t/(\bar{\pi}\pi_{t+1}^{gap}g_{t+1}))]\\
  c_{t+1,2} = \beta E_t[\lambda_t(s_t/(\bar{\pi}\pi_{t+1}^{gap}g_{t+1}))]\\  
\end{gather}
for $k=1,2$ where $k=1$ corresponds to the non-ZLB regime and $k=2$ corresponds to the ZLB regime.
\begin{gather}
c_{t} = c_{t,1}I + c_{t,2}(1-I) 
\end{gather}
for $j=1,2$ and where $I$ is defined by:
$$
\begin{cases}
  I = 1 & \text{ if } i > 1\\
  I = 0 & \text{ otherwise.}
\end{cases}
$$
%We use the functions, $V_l$, to determine the decisions rule though we do not approximate $V_l$ directly, because they inherit a kink associated with the ZLB constraint. Instead, we approximate functions, $V_{l,i}$, that are smoother and easier to approximate by specifying:
%\begin{gather}
%V_l = V_{l,1}I + V_{l,2}(1-I) 
%\end{gather}
%for $l \in \{\lambda, \pi\}$ and $j=1,2$ and where $I$ is defined by:
%\begin{gather}
%  I = 1 \text{ if } i > 1\\
%  \text{  } = 0 \text{ otherwise}
%\end{gather}
%In the above, $i = \max(1,i^*)$ where $i^*$ denotes the value of the notional rate derived from evaluating the functions $V_{l,1}$ and using (2). (For each variable, we use $j=1$ to denote the function associated with the regime with a positive nominal interest rate and $j=2$ to denote the function associated with the ZLB regime. \\
%Because the functions, $V_l$ depend directly on the nominal interest rate, we expect then to have a kink or non-differentiability. By contrast, the counterpart functions, $V_{l,j}$, that are indexed by the interest-rate regime do not depend on the current indicator function and thus are more likely to be smooth. \\
%Specifically, $V_{\pi,1}$ and $V_{\pi,2}$ are both described by (8) because the nominal interest rate does not appear in that equation. $V_{\lambda,1}$ is described by (6), but for the ZLB regime:
%\begin{gather}
%V_{\lambda,t,2} =  \beta E_t[(1/\lambda_{t+1})(s_t/(\bar{\pi}\pi_{t+1}^{gap}g_{t+1}))]\\  
%\end{gather}
%where $i_t$ is replaced by 1.
\end{comment}
\end{document}

